examples/steel/arraystructs/PointStruct.fst
@@ -22,8 +22,8 @@ let mk_point_f (x y: option int) (k: point_field): point_fields k = match k with
   | X -> x
   | Y -> y
   
-let mk_point (x y: Ghost.erased (option int)): Ghost.erased point =
-  Ghost.hide (on_domain point_field (mk_point_f (Ghost.reveal x) (Ghost.reveal y)))
+let mk_point (x y: option int): point =
+  on_domain point_field (mk_point_f x y)
 
 let _x = struct_field point_fields_pcm X
 let _y = struct_field point_fields_pcm Y
@@ -36,25 +36,25 @@ let point_without_x x y
 = ()
 
 let point_with_x x y
-: Lemma (struct_with_field point_fields_pcm X (Ghost.reveal x) (mk_point none y) `feq`
-         Ghost.reveal (mk_point x y))
+: Lemma (struct_with_field point_fields_pcm X x (mk_point None y) `feq`
+         mk_point x y)
   [SMTPat (mk_point x y)]
 = ()
 
 let point_without_y x y
-: Lemma (struct_without_field point_fields_pcm Y (mk_point x y) `feq` Ghost.reveal (mk_point x none))
+: Lemma (struct_without_field point_fields_pcm Y (mk_point x y) `feq` mk_point x None)
   [SMTPat (mk_point x y)]
 = ()
 
 let point_with_y x y
-: Lemma (struct_with_field point_fields_pcm Y (Ghost.reveal y) (mk_point x none) `feq`
-         Ghost.reveal (mk_point x y))
+: Lemma (struct_with_field point_fields_pcm Y y (mk_point x None) `feq`
+         mk_point x y)
   [SMTPat (mk_point x y)]
 = ()
 
 let addr_of_x #a #x #y p =
   let q = addr_of_struct_field p X (mk_point x y) in
-  A.change_equal_slprop (p `pts_to` _) (p `pts_to` mk_point none y);
+  A.change_equal_slprop (p `pts_to` _) (p `pts_to` mk_point None y);
   A.change_equal_slprop (q `pts_to` _) (q `pts_to` x);
   A.return q
   
@@ -64,7 +64,7 @@ let unaddr_of_x #a #x #y p q =
 
 let addr_of_y #a #x #y p =
   let q = addr_of_struct_field p Y (mk_point x y) in
-  A.change_equal_slprop (p `pts_to` _) (p `pts_to` mk_point x none);
+  A.change_equal_slprop (p `pts_to` _) (p `pts_to` mk_point x None);
   A.change_equal_slprop (q `pts_to` _) (q `pts_to` y);
   A.return q
 
